protobuf-shim/proofs/fstar/extraction/Protobuf.Reflect.Enums.fst
@@ -3,5 +3,13 @@ module Protobuf.Reflect.Enums
 open Core
 open FStar.Mul
 
+let impl__EnumDescriptor__hax_new (_: Prims.unit) =
+  { f__hax_placeholder = () <: Prims.unit } <: t_EnumDescriptor
+
 let impl__EnumDescriptor__new (#v_T: Type0) (file_descriptor: v_T) (index: usize) =
   { f__hax_placeholder = () <: Prims.unit } <: t_EnumDescriptor
+
+let impl__EnumDescriptor__value_by_index (self: t_EnumDescriptor) (index: usize) =
+  { Protobuf.Reflect.f__hax_placeholder = () <: Prims.unit }
+  <:
+  Protobuf.Reflect.t_EnumValueDescriptor
